\documentclass[11pt]{article}
\author{Lawrence Liu}
\usepackage{subcaption}
\usepackage{graphicx}
\usepackage{amsmath,amssymb,stmaryrd}
\usepackage{physics}
\usepackage{pdfpages}
\newcommand{\Laplace}{\mathscr{L}}
\setlength{\parskip}{\baselineskip}%
\setlength{\parindent}{0pt}%
\usepackage{xcolor}
\usepackage{listings}
\definecolor{backcolour}{rgb}{0.95,0.95,0.92}
\usepackage{amssymb}
\lstdefinestyle{mystyle}{
    backgroundcolor=\color{backcolour}}
\lstset{style=mystyle}
\title{Physics 115C HW 3}
\begin{document}
\maketitle
\section*{Problem 1}
\subsection*{(a)}
It would take $(-13.6\text{eV} - (-14.36 \text{eV})) = 0.76\text{eV}$ to remove one of the 
two electrons from the Hydrogen anion.
\subsection*{(b)}
\section*{Problem 2}
\subsection*{(a)}
We have that from the Virial theorem for a 
harmonic oscillator that
$$\langle T\rangle = \langle V\rangle$$
Therefore:
$$\langle T \rangle =  \frac{E_n}{2}$$
We have that our trial wavefunction is effectively the 
equal to the wavefunction for a harmonic oscillator with
$\omega=\lambda$. And since the energy of the ground state of a 
harmonic oscillator is given by
$$E_n = \hbar\omega\frac{1}{2}$$
We have that
$$\bra{\psi_{trial}}T\ket{\psi_{trial}} = \boxed{\frac{\hbar\lambda}{4}}$$.
\subsection*{(b)}
We shall prove that 
$$\int_{-\infty}^{\infty} x^{2n}e^{-ax^2}dx = \frac{\prod_{k=1}^n (2k-1)}{(2a)^n}\sqrt{\frac{\pi}{a}}$$
Through induction, for $n=1$ we have that 
$$\int_{-\infty}^{\infty} x^{2}e^{-ax^2}dx =\sqrt{\frac{\pi}{a}}\int_{-\infty}^{\infty} \sqrt{\frac{a}{\pi}}x^{2}e^{-\frac{1}{2}\frac{x^2}{\frac{1}{2a}}}dx $$
As we can see the integral is now the integral for the second moment of a gaussian with variance 
$\frac{1}{2a}$ centered around 0. Therefore we have that 
$$\int_{-\infty}^{\infty} x^{2}e^{-ax^2}dx =\frac{1}{2a}\sqrt{\frac{\pi}{a}}$$
Now we assume that the integral holds for $n=k$ and we shall prove that it holds for $n=k+1$.
We have that
\begin{align*}
    -\int_{-\infty}^{\infty} x^{2k+2}e^{-ax^2}dx &= \frac{d}{da}\int_{-\infty}^{\infty} x^{2k}e^{-ax^2}dx\\
    &= \frac{d}{da}\frac{\sqrt{\pi}\prod_{k=1}^n (2k-1)}{2^na^{n+\frac{1}{2}}}\\
    &= -\frac{\sqrt{\pi}(n+\frac{1}{2})\prod_{k=1}^n (2k-1)}{2^na^{n+\frac{1}{2}+1}}\\
    \int_{-\infty}^{\infty} x^{2k+2}e^{-ax^2}dx&= \boxed{\frac{\prod_{k=1}^{n+1} (2k-1)}{(2a)^{n+1}}\sqrt{\frac{\pi}{a}}}
\end{align*}
We have that 
\begin{align*}
    \bra{\psi_{trial}}V\ket{\psi_{trial}} &= \left(\frac{m\lambda}{\pi\hbar}\right)^\frac{1}{2} \int_{-\infty}^{\infty} kx^4 e^{-\frac{m\lambda}{\hbar}x^2}dx\\
    &= \boxed{\frac{3k}{2^2\left(\frac{m\lambda}{\hbar}\right)^2}}\\
\end{align*}
\subsection*{(c)}
We have that 
$$\bar{H} = \frac{\hbar \lambda}{4}+\frac{3k}{4\left(\frac{m\lambda}{\hbar}\right)^2}$$
Taking the derivative and setting it equal to 0 we have that:
\begin{align*}
    \frac{\hbar}{4} - \frac{2\cdot3k\hbar^2}{4m^2\lambda^3} &= 0\\
    \hbar &= \frac{2\cdot3k\hbar^2}{m^2\lambda^3}\\
    \lambda^3 &= \frac{2\cdot3k\hbar}{m^2}\\
    \lambda &= \boxed{\left(\frac{2\cdot3k\hbar}{m^2}\right)^\frac{1}{3}}
\end{align*}
\subsection*{(d)}
We thus have that for $\hbar = m = 1$ and $k=\frac{1}{2}$:
$$\lambda = 3^\frac{1}{3}$$
Therefore we have that 
$$\bar{H} =  \frac{3^\frac{1}{3}}{4}+\frac{3}{8\cdot3^\frac{2}{3}} = \boxed{0.540}$$
Which is $\boxed{2\%}$ away from the numerical value of $0.53$.
\section*{Problem 3}
\subsection*{(a)}
We have that 
$$
    \begin{pmatrix}
        \dot{c_1}\\
        \dot{c_2}\\
    \end{pmatrix}=
    \frac{1}{i\hbar}
    \begin{pmatrix}
        0 & \frac{\gamma}{2}e^{-i(\omega_{21}-\omega)t}\\
        \frac{\gamma}{2}e^{i(\omega_{21}-\omega)t} & 0\\
    \end{pmatrix}
    \begin{pmatrix}
        c_1\\
        c_2\\
    \end{pmatrix}
$$
When $\delta \omega = \omega_{21}-\omega$ we have that 
$$
    \begin{pmatrix}
        \dot{c_1}\\
        \dot{c_2}\\
    \end{pmatrix}=
    \frac{1}{i\hbar}
    \begin{pmatrix}
        0 & \frac{\gamma}{2}e^{-i\delta\omega t}\\
        \frac{\gamma}{2}e^{i\delta\omega t} & 0\\
    \end{pmatrix}
    \begin{pmatrix}
        c_1\\
        c_2\\
    \end{pmatrix}
$$
\subsection*{(b)}
We have that 
\begin{align*}
    \dot{c_2}&=\frac{1}{i\hbar}\frac{\gamma}{2}e^{i\delta\omega t}c_1\\
    \ddot{c_2}&=\frac{1}{i\hbar}\frac{\gamma}{2}e^{i\delta\omega t}\dot{c_1}+\frac{\delta\omega\gamma}{2\hbar}e^{i\delta\omega t}c_1\\
    &=-\frac{\gamma^2}{4\hbar^2}c_2+i\delta\omega \dot{c_2}\\
    \ddot{c_2}-i\delta\omega \dot{c_2}+\frac{\gamma^2}{4\hbar^2}c_2&=0
\end{align*}
\subsection*{(c)}
We have that the corresponding characteristic equation is
$$\lambda^2-i\delta\omega\lambda+\frac{\gamma^2}{4\hbar^2}=0$$
Therefore we have 
$$\lambda = \frac{i\delta\omega\pm\sqrt{-\delta\omega^2-\frac{\gamma^2}{\hbar^2}}}{2}$$
$$\lambda = i\frac{\delta\omega+\Omega}{2}$$
Where $\Omega = \sqrt{\delta\omega^2+\frac{\gamma^2}{\hbar^2}}$
Therefore we have that the solution is off the form 
$$c_2(t) = Ae^{i\frac{\delta\omega+\Omega}{2}t}+Be^{i\frac{\delta\omega-\Omega}{2}t}$$
Which we can rearage to:
$$c_2(t) = C_{+}e^{i\xi_+ t}+C_{-}e^{i\xi_- t}$$
Where $\xi_{\pm} = \frac{\delta\omega\pm\Omega}{2}$.
\subsection*{(d)}
We have that:
\begin{align*}
    c_2(0) &= 0\\
    C_{+}+C_{-} &= 0\\
    C_{-} &= -C_{+}\\
\end{align*}
Likewise we have that 
\begin{align*}
    c_1(0)  &= 1\\
    i\hbar\frac{2}{\gamma}\dot{c_2}(0) &= 1\\
    i\hbar\frac{2}{\gamma}\left(-i\xi_{+}C_{-}+i\xi_{-}C_{-}\right) &= 1\\
    \frac{2i\hbar}{\gamma}\left(\xi_{-}-\xi_{+}\right)C_{-} &= 1\\
    \frac{2i\hbar}{\gamma}\left(-\Omega\right)C_{-} &= 1\\
    C_{-} &= -\frac{\gamma}{2i\hbar\Omega}
\end{align*}
Therefore we have that
$$c_{2}(t) = \frac{\gamma}{2i\hbar\Omega}\left(e^{i\xi_{+}t}-e^{i\xi_{-}t}\right)$$
And thus we have that 
$$c_{2}^{*}(t) = \frac{-\gamma}{2i\hbar\Omega}\left(e^{-i\xi_{+}t}-e^{-i\xi_{-}t}\right)$$
\begin{align*}
    |c_{2}(t)|^2 &= \frac{\gamma^2}{4\hbar^2\Omega^2}\left(e^{i\xi_{+}t}-e^{i\xi_{-}t}\right)\left(e^{-i\xi_{+}t}-e^{-i\xi_{-}t}\right)\\
    &= \frac{\gamma^2}{4\hbar^2\Omega^2}\left(2-2\cos\left(\xi_{+}-\xi_{-}\right)t\right)\\
    &= \frac{\gamma^2}{2\hbar^2\Omega^2}\left(1-\cos\left(\Omega t\right)\right)\\
    &= \frac{\gamma^2}{\hbar^2\Omega^2}\sin^2\left(\frac{\Omega t}{2}\right)\\
\end{align*}
\subsection*{(e)}
The maximum value of $|c_2(t)|^2$ is $\frac{\gamma^2}{\hbar^2\Omega^2}$ which is reached when $\sin^2\left(\frac{\Omega t}{2}\right) = 1$.
We have that 
\begin{align*}
    \frac{\gamma^2}{\hbar^2\Omega^2} &= \frac{\gamma^2}{\hbar^2(\delta\omega^2+\frac{\gamma^2}{\hbar^2})}
\end{align*}
Therefore we can see that when $\delta\omega=0$, we recover back the result for the 
rabbi oscialltion at resonance, and for values of $\delta\omega\neq 0$ we have that 
$\delta\omega^2>0$ and thus $\frac{\gamma^2}{\hbar^2(\delta\omega^2+\frac{\gamma^2}{\hbar^2})}<1$.
\subsection*{(f)}
Since the particle can only take two possible states, 
we have that at equal superposition, we must have 
\begin{align*}
    |c_{2}(t)|^2 &= \frac{1}{2}\\
    \frac{\gamma^2}{\hbar^2\Omega^2}\sin^2\left(\frac{\Omega t}{2}\right) &= \frac{1}{2}\\
    \sin\left(\frac{\Omega t}{2}\right) &= \frac{\hbar \Omega}{\gamma\sqrt{2}}\\
    \frac{\Omega t}{2} &= \arcsin\left(\frac{\hbar \Omega}{\gamma\sqrt{2}}\right)\\
    t &= \frac{2}{\Omega}\arcsin\left(\frac{\hbar \Omega}{\gamma\sqrt{2}}\right)\\
\end{align*}
Thus we can see that the time it takes for the particle to reach equal superposition increases
as $|\delta\omega|$ increases and it takes longer than 
at resonance.
\section*{Problem 4}
\subsection*{(a)}
We have 

\end{document}